libcrux-ml-dsa/proofs/fstar/extraction/Libcrux_ml_dsa.Simd.Avx2.Arithmetic.fst
@@ -88,6 +88,35 @@ let montgomery_multiply_by_constant
   in
   Libcrux_intrinsics.Avx2.mm256_blend_epi32 (mk_i32 170) res02_shifted res13
 
+let montgomery_multiply_spec__i32_extended64_mul (x y: i32) : i64 =
+  (cast (x <: i32) <: i64) *! (cast (y <: i32) <: i64)
+
+let montgomery_multiply_spec (x y: i32) : i32 =
+  let x_mul_y:i64 = montgomery_multiply_spec__i32_extended64_mul x y in
+  let lhs:i32 = cast (x_mul_y >>! mk_i32 32 <: i64) <: i32 in
+  let rhs:i32 =
+    cast (((cast (cast (montgomery_multiply_spec__i32_extended64_mul (cast (x_mul_y <: i64) <: i32)
+                      (cast (Libcrux_ml_dsa.Simd.Traits.v_INVERSE_OF_MODULUS_MOD_MONTGOMERY_R <: u64
+                          )
+                        <:
+                        i32)
+                    <:
+                    i64)
+                <:
+                i32)
+            <:
+            i64) *!
+          (cast (Libcrux_ml_dsa.Simd.Traits.v_FIELD_MODULUS <: i32) <: i64)
+          <:
+          i64) >>!
+        mk_i32 32
+        <:
+        i64)
+    <:
+    i32
+  in
+  Core.Num.impl_i32__wrapping_sub lhs rhs
+
 [@@FStar.Tactics.postprocess_with ( Core_models.Core_arch.X86.Interpretations.Int_vec.Lemmas.flatten_circuit )]
 
 let montgomery_multiply (lhs rhs: Core_models.Abstractions.Bitvec.t_BitVec (mk_u64 256))
@@ -140,6 +169,8 @@ let montgomery_multiply (lhs rhs: Core_models.Abstractions.Bitvec.t_BitVec (mk_u
     Libcrux_intrinsics.Avx2.mm256_blend_epi32 (mk_i32 170) res02_shifted res13
   in
   lhs
+
+let hey: Lemma (e_ee_1__impl__to_i32x8 (montgomery_multiply lhs rhs) 0 == montgomery_multiply_spec (e_ee_1__impl__to_i32x8 lhs 0) (e_ee_1__impl__to_i32x8 rhs 0)) = ()
 
 let shift_left_then_reduce
       (v_SHIFT_BY: i32)
