fstar-helpers/core-models/proofs/fstar/extraction/Core_models.Abstractions.Bitvec.Int_vec_interp.fst
@@ -32,13 +32,21 @@ let e_ee_1__impl__to_i32x8 = e_ee_1__impl__to_i32x8'
 assume
 val e_ee_1__lemma_cancel_iv': x: Core_models.Abstractions.Funarr.t_FunArray (mk_u64 8) i32
   -> Lemma
-    (ensures
-      (e_ee_1__impl__to_i32x8 (e_ee_1__impl__from_i32x8 x
-            <:
-            Core_models.Abstractions.Bitvec.t_BitVec (mk_u64 256))
-        <:
-        Core_models.Abstractions.Funarr.t_FunArray (mk_u64 8) i32) ==
-      x)
+      (ensures
+        (e_ee_1__impl__to_i32x8 (e_ee_1__impl__from_i32x8 x
+              <:
+              Core_models.Abstractions.Bitvec.t_BitVec (mk_u64 256))
+          <:
+          Core_models.Abstractions.Funarr.t_FunArray (mk_u64 8) i32) ==
+        x)
+      [
+        SMTPat
+        (e_ee_1__impl__to_i32x8 (e_ee_1__impl__from_i32x8 x
+              <:
+              Core_models.Abstractions.Bitvec.t_BitVec (mk_u64 256))
+          <:
+          Core_models.Abstractions.Funarr.t_FunArray (mk_u64 8) i32)
+      ]
 
 unfold
 let e_ee_1__lemma_cancel_iv = e_ee_1__lemma_cancel_iv'
@@ -49,13 +57,21 @@ let e_ee_1__lemma_cancel_iv = e_ee_1__lemma_cancel_iv'
 assume
 val e_ee_1__lemma_cancel_bv': x: Core_models.Abstractions.Bitvec.t_BitVec (mk_u64 256)
   -> Lemma
-    (ensures
-      (e_ee_1__impl__from_i32x8 (e_ee_1__impl__to_i32x8 x
-            <:
-            Core_models.Abstractions.Funarr.t_FunArray (mk_u64 8) i32)
-        <:
-        Core_models.Abstractions.Bitvec.t_BitVec (mk_u64 256)) ==
-      x)
+      (ensures
+        (e_ee_1__impl__from_i32x8 (e_ee_1__impl__to_i32x8 x
+              <:
+              Core_models.Abstractions.Funarr.t_FunArray (mk_u64 8) i32)
+          <:
+          Core_models.Abstractions.Bitvec.t_BitVec (mk_u64 256)) ==
+        x)
+      [
+        SMTPat
+        (e_ee_1__impl__from_i32x8 (e_ee_1__impl__to_i32x8 x
+              <:
+              Core_models.Abstractions.Funarr.t_FunArray (mk_u64 8) i32)
+          <:
+          Core_models.Abstractions.Bitvec.t_BitVec (mk_u64 256))
+      ]
 
 unfold
 let e_ee_1__lemma_cancel_bv = e_ee_1__lemma_cancel_bv'
@@ -84,13 +100,21 @@ let e_ee_2__impl__to_i64x4 = e_ee_2__impl__to_i64x4'
 assume
 val e_ee_2__lemma_cancel_iv': x: Core_models.Abstractions.Funarr.t_FunArray (mk_u64 4) i64
   -> Lemma
-    (ensures
-      (e_ee_2__impl__to_i64x4 (e_ee_2__impl__from_i64x4 x
-            <:
-            Core_models.Abstractions.Bitvec.t_BitVec (mk_u64 256))
-        <:
-        Core_models.Abstractions.Funarr.t_FunArray (mk_u64 4) i64) ==
-      x)
+      (ensures
+        (e_ee_2__impl__to_i64x4 (e_ee_2__impl__from_i64x4 x
+              <:
+              Core_models.Abstractions.Bitvec.t_BitVec (mk_u64 256))
+          <:
+          Core_models.Abstractions.Funarr.t_FunArray (mk_u64 4) i64) ==
+        x)
+      [
+        SMTPat
+        (e_ee_2__impl__to_i64x4 (e_ee_2__impl__from_i64x4 x
+              <:
+              Core_models.Abstractions.Bitvec.t_BitVec (mk_u64 256))
+          <:
+          Core_models.Abstractions.Funarr.t_FunArray (mk_u64 4) i64)
+      ]
 
 unfold
 let e_ee_2__lemma_cancel_iv = e_ee_2__lemma_cancel_iv'
@@ -101,13 +125,21 @@ let e_ee_2__lemma_cancel_iv = e_ee_2__lemma_cancel_iv'
 assume
 val e_ee_2__lemma_cancel_bv': x: Core_models.Abstractions.Bitvec.t_BitVec (mk_u64 256)
   -> Lemma
-    (ensures
-      (e_ee_2__impl__from_i64x4 (e_ee_2__impl__to_i64x4 x
-            <:
-            Core_models.Abstractions.Funarr.t_FunArray (mk_u64 4) i64)
-        <:
-        Core_models.Abstractions.Bitvec.t_BitVec (mk_u64 256)) ==
-      x)
+      (ensures
+        (e_ee_2__impl__from_i64x4 (e_ee_2__impl__to_i64x4 x
+              <:
+              Core_models.Abstractions.Funarr.t_FunArray (mk_u64 4) i64)
+          <:
+          Core_models.Abstractions.Bitvec.t_BitVec (mk_u64 256)) ==
+        x)
+      [
+        SMTPat
+        (e_ee_2__impl__from_i64x4 (e_ee_2__impl__to_i64x4 x
+              <:
+              Core_models.Abstractions.Funarr.t_FunArray (mk_u64 4) i64)
+          <:
+          Core_models.Abstractions.Bitvec.t_BitVec (mk_u64 256))
+      ]
 
 unfold
 let e_ee_2__lemma_cancel_bv = e_ee_2__lemma_cancel_bv'
@@ -136,13 +168,21 @@ let e_ee_3__impl__to_i16x16 = e_ee_3__impl__to_i16x16'
 assume
 val e_ee_3__lemma_cancel_iv': x: Core_models.Abstractions.Funarr.t_FunArray (mk_u64 16) i16
   -> Lemma
-    (ensures
-      (e_ee_3__impl__to_i16x16 (e_ee_3__impl__from_i16x16 x
-            <:
-            Core_models.Abstractions.Bitvec.t_BitVec (mk_u64 256))
-        <:
-        Core_models.Abstractions.Funarr.t_FunArray (mk_u64 16) i16) ==
-      x)
+      (ensures
+        (e_ee_3__impl__to_i16x16 (e_ee_3__impl__from_i16x16 x
+              <:
+              Core_models.Abstractions.Bitvec.t_BitVec (mk_u64 256))
+          <:
+          Core_models.Abstractions.Funarr.t_FunArray (mk_u64 16) i16) ==
+        x)
+      [
+        SMTPat
+        (e_ee_3__impl__to_i16x16 (e_ee_3__impl__from_i16x16 x
+              <:
+              Core_models.Abstractions.Bitvec.t_BitVec (mk_u64 256))
+          <:
+          Core_models.Abstractions.Funarr.t_FunArray (mk_u64 16) i16)
+      ]
 
 unfold
 let e_ee_3__lemma_cancel_iv = e_ee_3__lemma_cancel_iv'
@@ -153,13 +193,21 @@ let e_ee_3__lemma_cancel_iv = e_ee_3__lemma_cancel_iv'
 assume
 val e_ee_3__lemma_cancel_bv': x: Core_models.Abstractions.Bitvec.t_BitVec (mk_u64 256)
   -> Lemma
-    (ensures
-      (e_ee_3__impl__from_i16x16 (e_ee_3__impl__to_i16x16 x
-            <:
-            Core_models.Abstractions.Funarr.t_FunArray (mk_u64 16) i16)
-        <:
-        Core_models.Abstractions.Bitvec.t_BitVec (mk_u64 256)) ==
-      x)
+      (ensures
+        (e_ee_3__impl__from_i16x16 (e_ee_3__impl__to_i16x16 x
+              <:
+              Core_models.Abstractions.Funarr.t_FunArray (mk_u64 16) i16)
+          <:
+          Core_models.Abstractions.Bitvec.t_BitVec (mk_u64 256)) ==
+        x)
+      [
+        SMTPat
+        (e_ee_3__impl__from_i16x16 (e_ee_3__impl__to_i16x16 x
+              <:
+              Core_models.Abstractions.Funarr.t_FunArray (mk_u64 16) i16)
+          <:
+          Core_models.Abstractions.Bitvec.t_BitVec (mk_u64 256))
+      ]
 
 unfold
 let e_ee_3__lemma_cancel_bv = e_ee_3__lemma_cancel_bv'
@@ -188,13 +236,21 @@ let e_ee_4__impl__to_i128x2 = e_ee_4__impl__to_i128x2'
 assume
 val e_ee_4__lemma_cancel_iv': x: Core_models.Abstractions.Funarr.t_FunArray (mk_u64 2) i128
   -> Lemma
-    (ensures
-      (e_ee_4__impl__to_i128x2 (e_ee_4__impl__from_i128x2 x
-            <:
-            Core_models.Abstractions.Bitvec.t_BitVec (mk_u64 256))
-        <:
-        Core_models.Abstractions.Funarr.t_FunArray (mk_u64 2) i128) ==
-      x)
+      (ensures
+        (e_ee_4__impl__to_i128x2 (e_ee_4__impl__from_i128x2 x
+              <:
+              Core_models.Abstractions.Bitvec.t_BitVec (mk_u64 256))
+          <:
+          Core_models.Abstractions.Funarr.t_FunArray (mk_u64 2) i128) ==
+        x)
+      [
+        SMTPat
+        (e_ee_4__impl__to_i128x2 (e_ee_4__impl__from_i128x2 x
+              <:
+              Core_models.Abstractions.Bitvec.t_BitVec (mk_u64 256))
+          <:
+          Core_models.Abstractions.Funarr.t_FunArray (mk_u64 2) i128)
+      ]
 
 unfold
 let e_ee_4__lemma_cancel_iv = e_ee_4__lemma_cancel_iv'
@@ -205,13 +261,21 @@ let e_ee_4__lemma_cancel_iv = e_ee_4__lemma_cancel_iv'
 assume
 val e_ee_4__lemma_cancel_bv': x: Core_models.Abstractions.Bitvec.t_BitVec (mk_u64 256)
   -> Lemma
-    (ensures
-      (e_ee_4__impl__from_i128x2 (e_ee_4__impl__to_i128x2 x
-            <:
-            Core_models.Abstractions.Funarr.t_FunArray (mk_u64 2) i128)
-        <:
-        Core_models.Abstractions.Bitvec.t_BitVec (mk_u64 256)) ==
-      x)
+      (ensures
+        (e_ee_4__impl__from_i128x2 (e_ee_4__impl__to_i128x2 x
+              <:
+              Core_models.Abstractions.Funarr.t_FunArray (mk_u64 2) i128)
+          <:
+          Core_models.Abstractions.Bitvec.t_BitVec (mk_u64 256)) ==
+        x)
+      [
+        SMTPat
+        (e_ee_4__impl__from_i128x2 (e_ee_4__impl__to_i128x2 x
+              <:
+              Core_models.Abstractions.Funarr.t_FunArray (mk_u64 2) i128)
+          <:
+          Core_models.Abstractions.Bitvec.t_BitVec (mk_u64 256))
+      ]
 
 unfold
 let e_ee_4__lemma_cancel_bv = e_ee_4__lemma_cancel_bv'
@@ -240,13 +304,21 @@ let e_ee_5__impl__to_i8x32 = e_ee_5__impl__to_i8x32'
 assume
 val e_ee_5__lemma_cancel_iv': x: Core_models.Abstractions.Funarr.t_FunArray (mk_u64 32) i8
   -> Lemma
-    (ensures
-      (e_ee_5__impl__to_i8x32 (e_ee_5__impl__from_i8x32 x
-            <:
-            Core_models.Abstractions.Bitvec.t_BitVec (mk_u64 256))
-        <:
-        Core_models.Abstractions.Funarr.t_FunArray (mk_u64 32) i8) ==
-      x)
+      (ensures
+        (e_ee_5__impl__to_i8x32 (e_ee_5__impl__from_i8x32 x
+              <:
+              Core_models.Abstractions.Bitvec.t_BitVec (mk_u64 256))
+          <:
+          Core_models.Abstractions.Funarr.t_FunArray (mk_u64 32) i8) ==
+        x)
+      [
+        SMTPat
+        (e_ee_5__impl__to_i8x32 (e_ee_5__impl__from_i8x32 x
+              <:
+              Core_models.Abstractions.Bitvec.t_BitVec (mk_u64 256))
+          <:
+          Core_models.Abstractions.Funarr.t_FunArray (mk_u64 32) i8)
+      ]
 
 unfold
 let e_ee_5__lemma_cancel_iv = e_ee_5__lemma_cancel_iv'
@@ -257,13 +329,21 @@ let e_ee_5__lemma_cancel_iv = e_ee_5__lemma_cancel_iv'
 assume
 val e_ee_5__lemma_cancel_bv': x: Core_models.Abstractions.Bitvec.t_BitVec (mk_u64 256)
   -> Lemma
-    (ensures
-      (e_ee_5__impl__from_i8x32 (e_ee_5__impl__to_i8x32 x
-            <:
-            Core_models.Abstractions.Funarr.t_FunArray (mk_u64 32) i8)
-        <:
-        Core_models.Abstractions.Bitvec.t_BitVec (mk_u64 256)) ==
-      x)
+      (ensures
+        (e_ee_5__impl__from_i8x32 (e_ee_5__impl__to_i8x32 x
+              <:
+              Core_models.Abstractions.Funarr.t_FunArray (mk_u64 32) i8)
+          <:
+          Core_models.Abstractions.Bitvec.t_BitVec (mk_u64 256)) ==
+        x)
+      [
+        SMTPat
+        (e_ee_5__impl__from_i8x32 (e_ee_5__impl__to_i8x32 x
+              <:
+              Core_models.Abstractions.Funarr.t_FunArray (mk_u64 32) i8)
+          <:
+          Core_models.Abstractions.Bitvec.t_BitVec (mk_u64 256))
+      ]
 
 unfold
 let e_ee_5__lemma_cancel_bv = e_ee_5__lemma_cancel_bv'
@@ -292,13 +372,21 @@ let e_ee_6__impl__to_u32x8 = e_ee_6__impl__to_u32x8'
 assume
 val e_ee_6__lemma_cancel_iv': x: Core_models.Abstractions.Funarr.t_FunArray (mk_u64 8) u32
   -> Lemma
-    (ensures
-      (e_ee_6__impl__to_u32x8 (e_ee_6__impl__from_u32x8 x
-            <:
-            Core_models.Abstractions.Bitvec.t_BitVec (mk_u64 256))
-        <:
-        Core_models.Abstractions.Funarr.t_FunArray (mk_u64 8) u32) ==
-      x)
+      (ensures
+        (e_ee_6__impl__to_u32x8 (e_ee_6__impl__from_u32x8 x
+              <:
+              Core_models.Abstractions.Bitvec.t_BitVec (mk_u64 256))
+          <:
+          Core_models.Abstractions.Funarr.t_FunArray (mk_u64 8) u32) ==
+        x)
+      [
+        SMTPat
+        (e_ee_6__impl__to_u32x8 (e_ee_6__impl__from_u32x8 x
+              <:
+              Core_models.Abstractions.Bitvec.t_BitVec (mk_u64 256))
+          <:
+          Core_models.Abstractions.Funarr.t_FunArray (mk_u64 8) u32)
+      ]
 
 unfold
 let e_ee_6__lemma_cancel_iv = e_ee_6__lemma_cancel_iv'
@@ -309,13 +397,21 @@ let e_ee_6__lemma_cancel_iv = e_ee_6__lemma_cancel_iv'
 assume
 val e_ee_6__lemma_cancel_bv': x: Core_models.Abstractions.Bitvec.t_BitVec (mk_u64 256)
   -> Lemma
-    (ensures
-      (e_ee_6__impl__from_u32x8 (e_ee_6__impl__to_u32x8 x
-            <:
-            Core_models.Abstractions.Funarr.t_FunArray (mk_u64 8) u32)
-        <:
-        Core_models.Abstractions.Bitvec.t_BitVec (mk_u64 256)) ==
-      x)
+      (ensures
+        (e_ee_6__impl__from_u32x8 (e_ee_6__impl__to_u32x8 x
+              <:
+              Core_models.Abstractions.Funarr.t_FunArray (mk_u64 8) u32)
+          <:
+          Core_models.Abstractions.Bitvec.t_BitVec (mk_u64 256)) ==
+        x)
+      [
+        SMTPat
+        (e_ee_6__impl__from_u32x8 (e_ee_6__impl__to_u32x8 x
+              <:
+              Core_models.Abstractions.Funarr.t_FunArray (mk_u64 8) u32)
+          <:
+          Core_models.Abstractions.Bitvec.t_BitVec (mk_u64 256))
+      ]
 
 unfold
 let e_ee_6__lemma_cancel_bv = e_ee_6__lemma_cancel_bv'
@@ -344,13 +440,21 @@ let e_ee_7__impl__to_u64x4 = e_ee_7__impl__to_u64x4'
 assume
 val e_ee_7__lemma_cancel_iv': x: Core_models.Abstractions.Funarr.t_FunArray (mk_u64 4) u64
   -> Lemma
-    (ensures
-      (e_ee_7__impl__to_u64x4 (e_ee_7__impl__from_u64x4 x
-            <:
-            Core_models.Abstractions.Bitvec.t_BitVec (mk_u64 256))
-        <:
-        Core_models.Abstractions.Funarr.t_FunArray (mk_u64 4) u64) ==
-      x)
+      (ensures
+        (e_ee_7__impl__to_u64x4 (e_ee_7__impl__from_u64x4 x
+              <:
+              Core_models.Abstractions.Bitvec.t_BitVec (mk_u64 256))
+          <:
+          Core_models.Abstractions.Funarr.t_FunArray (mk_u64 4) u64) ==
+        x)
+      [
+        SMTPat
+        (e_ee_7__impl__to_u64x4 (e_ee_7__impl__from_u64x4 x
+              <:
+              Core_models.Abstractions.Bitvec.t_BitVec (mk_u64 256))
+          <:
+          Core_models.Abstractions.Funarr.t_FunArray (mk_u64 4) u64)
+      ]
 
 unfold
 let e_ee_7__lemma_cancel_iv = e_ee_7__lemma_cancel_iv'
@@ -361,13 +465,21 @@ let e_ee_7__lemma_cancel_iv = e_ee_7__lemma_cancel_iv'
 assume
 val e_ee_7__lemma_cancel_bv': x: Core_models.Abstractions.Bitvec.t_BitVec (mk_u64 256)
   -> Lemma
-    (ensures
-      (e_ee_7__impl__from_u64x4 (e_ee_7__impl__to_u64x4 x
-            <:
-            Core_models.Abstractions.Funarr.t_FunArray (mk_u64 4) u64)
-        <:
-        Core_models.Abstractions.Bitvec.t_BitVec (mk_u64 256)) ==
-      x)
+      (ensures
+        (e_ee_7__impl__from_u64x4 (e_ee_7__impl__to_u64x4 x
+              <:
+              Core_models.Abstractions.Funarr.t_FunArray (mk_u64 4) u64)
+          <:
+          Core_models.Abstractions.Bitvec.t_BitVec (mk_u64 256)) ==
+        x)
+      [
+        SMTPat
+        (e_ee_7__impl__from_u64x4 (e_ee_7__impl__to_u64x4 x
+              <:
+              Core_models.Abstractions.Funarr.t_FunArray (mk_u64 4) u64)
+          <:
+          Core_models.Abstractions.Bitvec.t_BitVec (mk_u64 256))
+      ]
 
 unfold
 let e_ee_7__lemma_cancel_bv = e_ee_7__lemma_cancel_bv'
@@ -396,13 +508,21 @@ let e_ee_8__impl__to_u16x16 = e_ee_8__impl__to_u16x16'
 assume
 val e_ee_8__lemma_cancel_iv': x: Core_models.Abstractions.Funarr.t_FunArray (mk_u64 16) u16
   -> Lemma
-    (ensures
-      (e_ee_8__impl__to_u16x16 (e_ee_8__impl__from_u16x16 x
-            <:
-            Core_models.Abstractions.Bitvec.t_BitVec (mk_u64 256))
-        <:
-        Core_models.Abstractions.Funarr.t_FunArray (mk_u64 16) u16) ==
-      x)
+      (ensures
+        (e_ee_8__impl__to_u16x16 (e_ee_8__impl__from_u16x16 x
+              <:
+              Core_models.Abstractions.Bitvec.t_BitVec (mk_u64 256))
+          <:
+          Core_models.Abstractions.Funarr.t_FunArray (mk_u64 16) u16) ==
+        x)
+      [
+        SMTPat
+        (e_ee_8__impl__to_u16x16 (e_ee_8__impl__from_u16x16 x
+              <:
+              Core_models.Abstractions.Bitvec.t_BitVec (mk_u64 256))
+          <:
+          Core_models.Abstractions.Funarr.t_FunArray (mk_u64 16) u16)
+      ]
 
 unfold
 let e_ee_8__lemma_cancel_iv = e_ee_8__lemma_cancel_iv'
@@ -413,13 +533,21 @@ let e_ee_8__lemma_cancel_iv = e_ee_8__lemma_cancel_iv'
 assume
 val e_ee_8__lemma_cancel_bv': x: Core_models.Abstractions.Bitvec.t_BitVec (mk_u64 256)
   -> Lemma
-    (ensures
-      (e_ee_8__impl__from_u16x16 (e_ee_8__impl__to_u16x16 x
-            <:
-            Core_models.Abstractions.Funarr.t_FunArray (mk_u64 16) u16)
-        <:
-        Core_models.Abstractions.Bitvec.t_BitVec (mk_u64 256)) ==
-      x)
+      (ensures
+        (e_ee_8__impl__from_u16x16 (e_ee_8__impl__to_u16x16 x
+              <:
+              Core_models.Abstractions.Funarr.t_FunArray (mk_u64 16) u16)
+          <:
+          Core_models.Abstractions.Bitvec.t_BitVec (mk_u64 256)) ==
+        x)
+      [
+        SMTPat
+        (e_ee_8__impl__from_u16x16 (e_ee_8__impl__to_u16x16 x
+              <:
+              Core_models.Abstractions.Funarr.t_FunArray (mk_u64 16) u16)
+          <:
+          Core_models.Abstractions.Bitvec.t_BitVec (mk_u64 256))
+      ]
 
 unfold
 let e_ee_8__lemma_cancel_bv = e_ee_8__lemma_cancel_bv'
@@ -448,13 +576,21 @@ let e_ee_9__impl__to_i32x4 = e_ee_9__impl__to_i32x4'
 assume
 val e_ee_9__lemma_cancel_iv': x: Core_models.Abstractions.Funarr.t_FunArray (mk_u64 4) i32
   -> Lemma
-    (ensures
-      (e_ee_9__impl__to_i32x4 (e_ee_9__impl__from_i32x4 x
-            <:
-            Core_models.Abstractions.Bitvec.t_BitVec (mk_u64 128))
-        <:
-        Core_models.Abstractions.Funarr.t_FunArray (mk_u64 4) i32) ==
-      x)
+      (ensures
+        (e_ee_9__impl__to_i32x4 (e_ee_9__impl__from_i32x4 x
+              <:
+              Core_models.Abstractions.Bitvec.t_BitVec (mk_u64 128))
+          <:
+          Core_models.Abstractions.Funarr.t_FunArray (mk_u64 4) i32) ==
+        x)
+      [
+        SMTPat
+        (e_ee_9__impl__to_i32x4 (e_ee_9__impl__from_i32x4 x
+              <:
+              Core_models.Abstractions.Bitvec.t_BitVec (mk_u64 128))
+          <:
+          Core_models.Abstractions.Funarr.t_FunArray (mk_u64 4) i32)
+      ]
 
 unfold
 let e_ee_9__lemma_cancel_iv = e_ee_9__lemma_cancel_iv'
@@ -465,13 +601,21 @@ let e_ee_9__lemma_cancel_iv = e_ee_9__lemma_cancel_iv'
 assume
 val e_ee_9__lemma_cancel_bv': x: Core_models.Abstractions.Bitvec.t_BitVec (mk_u64 128)
   -> Lemma
-    (ensures
-      (e_ee_9__impl__from_i32x4 (e_ee_9__impl__to_i32x4 x
-            <:
-            Core_models.Abstractions.Funarr.t_FunArray (mk_u64 4) i32)
-        <:
-        Core_models.Abstractions.Bitvec.t_BitVec (mk_u64 128)) ==
-      x)
+      (ensures
+        (e_ee_9__impl__from_i32x4 (e_ee_9__impl__to_i32x4 x
+              <:
+              Core_models.Abstractions.Funarr.t_FunArray (mk_u64 4) i32)
+          <:
+          Core_models.Abstractions.Bitvec.t_BitVec (mk_u64 128)) ==
+        x)
+      [
+        SMTPat
+        (e_ee_9__impl__from_i32x4 (e_ee_9__impl__to_i32x4 x
+              <:
+              Core_models.Abstractions.Funarr.t_FunArray (mk_u64 4) i32)
+          <:
+          Core_models.Abstractions.Bitvec.t_BitVec (mk_u64 128))
+      ]
 
 unfold
 let e_ee_9__lemma_cancel_bv = e_ee_9__lemma_cancel_bv'
@@ -500,13 +644,21 @@ let e_ee_10__impl__to_i64x2 = e_ee_10__impl__to_i64x2'
 assume
 val e_ee_10__lemma_cancel_iv': x: Core_models.Abstractions.Funarr.t_FunArray (mk_u64 2) i64
   -> Lemma
-    (ensures
-      (e_ee_10__impl__to_i64x2 (e_ee_10__impl__from_i64x2 x
-            <:
-            Core_models.Abstractions.Bitvec.t_BitVec (mk_u64 128))
-        <:
-        Core_models.Abstractions.Funarr.t_FunArray (mk_u64 2) i64) ==
-      x)
+      (ensures
+        (e_ee_10__impl__to_i64x2 (e_ee_10__impl__from_i64x2 x
+              <:
+              Core_models.Abstractions.Bitvec.t_BitVec (mk_u64 128))
+          <:
+          Core_models.Abstractions.Funarr.t_FunArray (mk_u64 2) i64) ==
+        x)
+      [
+        SMTPat
+        (e_ee_10__impl__to_i64x2 (e_ee_10__impl__from_i64x2 x
+              <:
+              Core_models.Abstractions.Bitvec.t_BitVec (mk_u64 128))
+          <:
+          Core_models.Abstractions.Funarr.t_FunArray (mk_u64 2) i64)
+      ]
 
 unfold
 let e_ee_10__lemma_cancel_iv = e_ee_10__lemma_cancel_iv'
@@ -517,13 +669,21 @@ let e_ee_10__lemma_cancel_iv = e_ee_10__lemma_cancel_iv'
 assume
 val e_ee_10__lemma_cancel_bv': x: Core_models.Abstractions.Bitvec.t_BitVec (mk_u64 128)
   -> Lemma
-    (ensures
-      (e_ee_10__impl__from_i64x2 (e_ee_10__impl__to_i64x2 x
-            <:
-            Core_models.Abstractions.Funarr.t_FunArray (mk_u64 2) i64)
-        <:
-        Core_models.Abstractions.Bitvec.t_BitVec (mk_u64 128)) ==
-      x)
+      (ensures
+        (e_ee_10__impl__from_i64x2 (e_ee_10__impl__to_i64x2 x
+              <:
+              Core_models.Abstractions.Funarr.t_FunArray (mk_u64 2) i64)
+          <:
+          Core_models.Abstractions.Bitvec.t_BitVec (mk_u64 128)) ==
+        x)
+      [
+        SMTPat
+        (e_ee_10__impl__from_i64x2 (e_ee_10__impl__to_i64x2 x
+              <:
+              Core_models.Abstractions.Funarr.t_FunArray (mk_u64 2) i64)
+          <:
+          Core_models.Abstractions.Bitvec.t_BitVec (mk_u64 128))
+      ]
 
 unfold
 let e_ee_10__lemma_cancel_bv = e_ee_10__lemma_cancel_bv'
@@ -552,13 +712,21 @@ let e_ee_11__impl__to_i16x8 = e_ee_11__impl__to_i16x8'
 assume
 val e_ee_11__lemma_cancel_iv': x: Core_models.Abstractions.Funarr.t_FunArray (mk_u64 8) i16
   -> Lemma
-    (ensures
-      (e_ee_11__impl__to_i16x8 (e_ee_11__impl__from_i16x8 x
-            <:
-            Core_models.Abstractions.Bitvec.t_BitVec (mk_u64 128))
-        <:
-        Core_models.Abstractions.Funarr.t_FunArray (mk_u64 8) i16) ==
-      x)
+      (ensures
+        (e_ee_11__impl__to_i16x8 (e_ee_11__impl__from_i16x8 x
+              <:
+              Core_models.Abstractions.Bitvec.t_BitVec (mk_u64 128))
+          <:
+          Core_models.Abstractions.Funarr.t_FunArray (mk_u64 8) i16) ==
+        x)
+      [
+        SMTPat
+        (e_ee_11__impl__to_i16x8 (e_ee_11__impl__from_i16x8 x
+              <:
+              Core_models.Abstractions.Bitvec.t_BitVec (mk_u64 128))
+          <:
+          Core_models.Abstractions.Funarr.t_FunArray (mk_u64 8) i16)
+      ]
 
 unfold
 let e_ee_11__lemma_cancel_iv = e_ee_11__lemma_cancel_iv'
@@ -569,13 +737,21 @@ let e_ee_11__lemma_cancel_iv = e_ee_11__lemma_cancel_iv'
 assume
 val e_ee_11__lemma_cancel_bv': x: Core_models.Abstractions.Bitvec.t_BitVec (mk_u64 128)
   -> Lemma
-    (ensures
-      (e_ee_11__impl__from_i16x8 (e_ee_11__impl__to_i16x8 x
-            <:
-            Core_models.Abstractions.Funarr.t_FunArray (mk_u64 8) i16)
-        <:
-        Core_models.Abstractions.Bitvec.t_BitVec (mk_u64 128)) ==
-      x)
+      (ensures
+        (e_ee_11__impl__from_i16x8 (e_ee_11__impl__to_i16x8 x
+              <:
+              Core_models.Abstractions.Funarr.t_FunArray (mk_u64 8) i16)
+          <:
+          Core_models.Abstractions.Bitvec.t_BitVec (mk_u64 128)) ==
+        x)
+      [
+        SMTPat
+        (e_ee_11__impl__from_i16x8 (e_ee_11__impl__to_i16x8 x
+              <:
+              Core_models.Abstractions.Funarr.t_FunArray (mk_u64 8) i16)
+          <:
+          Core_models.Abstractions.Bitvec.t_BitVec (mk_u64 128))
+      ]
 
 unfold
 let e_ee_11__lemma_cancel_bv = e_ee_11__lemma_cancel_bv'
@@ -604,13 +780,21 @@ let e_ee_12__impl__to_i128x1 = e_ee_12__impl__to_i128x1'
 assume
 val e_ee_12__lemma_cancel_iv': x: Core_models.Abstractions.Funarr.t_FunArray (mk_u64 1) i128
   -> Lemma
-    (ensures
-      (e_ee_12__impl__to_i128x1 (e_ee_12__impl__from_i128x1 x
-            <:
-            Core_models.Abstractions.Bitvec.t_BitVec (mk_u64 128))
-        <:
-        Core_models.Abstractions.Funarr.t_FunArray (mk_u64 1) i128) ==
-      x)
+      (ensures
+        (e_ee_12__impl__to_i128x1 (e_ee_12__impl__from_i128x1 x
+              <:
+              Core_models.Abstractions.Bitvec.t_BitVec (mk_u64 128))
+          <:
+          Core_models.Abstractions.Funarr.t_FunArray (mk_u64 1) i128) ==
+        x)
+      [
+        SMTPat
+        (e_ee_12__impl__to_i128x1 (e_ee_12__impl__from_i128x1 x
+              <:
+              Core_models.Abstractions.Bitvec.t_BitVec (mk_u64 128))
+          <:
+          Core_models.Abstractions.Funarr.t_FunArray (mk_u64 1) i128)
+      ]
 
 unfold
 let e_ee_12__lemma_cancel_iv = e_ee_12__lemma_cancel_iv'
@@ -621,13 +805,21 @@ let e_ee_12__lemma_cancel_iv = e_ee_12__lemma_cancel_iv'
 assume
 val e_ee_12__lemma_cancel_bv': x: Core_models.Abstractions.Bitvec.t_BitVec (mk_u64 128)
   -> Lemma
-    (ensures
-      (e_ee_12__impl__from_i128x1 (e_ee_12__impl__to_i128x1 x
-            <:
-            Core_models.Abstractions.Funarr.t_FunArray (mk_u64 1) i128)
-        <:
-        Core_models.Abstractions.Bitvec.t_BitVec (mk_u64 128)) ==
-      x)
+      (ensures
+        (e_ee_12__impl__from_i128x1 (e_ee_12__impl__to_i128x1 x
+              <:
+              Core_models.Abstractions.Funarr.t_FunArray (mk_u64 1) i128)
+          <:
+          Core_models.Abstractions.Bitvec.t_BitVec (mk_u64 128)) ==
+        x)
+      [
+        SMTPat
+        (e_ee_12__impl__from_i128x1 (e_ee_12__impl__to_i128x1 x
+              <:
+              Core_models.Abstractions.Funarr.t_FunArray (mk_u64 1) i128)
+          <:
+          Core_models.Abstractions.Bitvec.t_BitVec (mk_u64 128))
+      ]
 
 unfold
 let e_ee_12__lemma_cancel_bv = e_ee_12__lemma_cancel_bv'
@@ -656,13 +848,21 @@ let e_ee_13__impl__to_i8x16 = e_ee_13__impl__to_i8x16'
 assume
 val e_ee_13__lemma_cancel_iv': x: Core_models.Abstractions.Funarr.t_FunArray (mk_u64 16) i8
   -> Lemma
-    (ensures
-      (e_ee_13__impl__to_i8x16 (e_ee_13__impl__from_i8x16 x
-            <:
-            Core_models.Abstractions.Bitvec.t_BitVec (mk_u64 128))
-        <:
-        Core_models.Abstractions.Funarr.t_FunArray (mk_u64 16) i8) ==
-      x)
+      (ensures
+        (e_ee_13__impl__to_i8x16 (e_ee_13__impl__from_i8x16 x
+              <:
+              Core_models.Abstractions.Bitvec.t_BitVec (mk_u64 128))
+          <:
+          Core_models.Abstractions.Funarr.t_FunArray (mk_u64 16) i8) ==
+        x)
+      [
+        SMTPat
+        (e_ee_13__impl__to_i8x16 (e_ee_13__impl__from_i8x16 x
+              <:
+              Core_models.Abstractions.Bitvec.t_BitVec (mk_u64 128))
+          <:
+          Core_models.Abstractions.Funarr.t_FunArray (mk_u64 16) i8)
+      ]
 
 unfold
 let e_ee_13__lemma_cancel_iv = e_ee_13__lemma_cancel_iv'
@@ -673,13 +873,21 @@ let e_ee_13__lemma_cancel_iv = e_ee_13__lemma_cancel_iv'
 assume
 val e_ee_13__lemma_cancel_bv': x: Core_models.Abstractions.Bitvec.t_BitVec (mk_u64 128)
   -> Lemma
-    (ensures
-      (e_ee_13__impl__from_i8x16 (e_ee_13__impl__to_i8x16 x
-            <:
-            Core_models.Abstractions.Funarr.t_FunArray (mk_u64 16) i8)
-        <:
-        Core_models.Abstractions.Bitvec.t_BitVec (mk_u64 128)) ==
-      x)
+      (ensures
+        (e_ee_13__impl__from_i8x16 (e_ee_13__impl__to_i8x16 x
+              <:
+              Core_models.Abstractions.Funarr.t_FunArray (mk_u64 16) i8)
+          <:
+          Core_models.Abstractions.Bitvec.t_BitVec (mk_u64 128)) ==
+        x)
+      [
+        SMTPat
+        (e_ee_13__impl__from_i8x16 (e_ee_13__impl__to_i8x16 x
+              <:
+              Core_models.Abstractions.Funarr.t_FunArray (mk_u64 16) i8)
+          <:
+          Core_models.Abstractions.Bitvec.t_BitVec (mk_u64 128))
+      ]
 
 unfold
 let e_ee_13__lemma_cancel_bv = e_ee_13__lemma_cancel_bv'
@@ -708,13 +916,21 @@ let e_ee_14__impl__to_u32x4 = e_ee_14__impl__to_u32x4'
 assume
 val e_ee_14__lemma_cancel_iv': x: Core_models.Abstractions.Funarr.t_FunArray (mk_u64 4) u32
   -> Lemma
-    (ensures
-      (e_ee_14__impl__to_u32x4 (e_ee_14__impl__from_u32x4 x
-            <:
-            Core_models.Abstractions.Bitvec.t_BitVec (mk_u64 128))
-        <:
-        Core_models.Abstractions.Funarr.t_FunArray (mk_u64 4) u32) ==
-      x)
+      (ensures
+        (e_ee_14__impl__to_u32x4 (e_ee_14__impl__from_u32x4 x
+              <:
+              Core_models.Abstractions.Bitvec.t_BitVec (mk_u64 128))
+          <:
+          Core_models.Abstractions.Funarr.t_FunArray (mk_u64 4) u32) ==
+        x)
+      [
+        SMTPat
+        (e_ee_14__impl__to_u32x4 (e_ee_14__impl__from_u32x4 x
+              <:
+              Core_models.Abstractions.Bitvec.t_BitVec (mk_u64 128))
+          <:
+          Core_models.Abstractions.Funarr.t_FunArray (mk_u64 4) u32)
+      ]
 
 unfold
 let e_ee_14__lemma_cancel_iv = e_ee_14__lemma_cancel_iv'
@@ -725,13 +941,21 @@ let e_ee_14__lemma_cancel_iv = e_ee_14__lemma_cancel_iv'
 assume
 val e_ee_14__lemma_cancel_bv': x: Core_models.Abstractions.Bitvec.t_BitVec (mk_u64 128)
   -> Lemma
-    (ensures
-      (e_ee_14__impl__from_u32x4 (e_ee_14__impl__to_u32x4 x
-            <:
-            Core_models.Abstractions.Funarr.t_FunArray (mk_u64 4) u32)
-        <:
-        Core_models.Abstractions.Bitvec.t_BitVec (mk_u64 128)) ==
-      x)
+      (ensures
+        (e_ee_14__impl__from_u32x4 (e_ee_14__impl__to_u32x4 x
+              <:
+              Core_models.Abstractions.Funarr.t_FunArray (mk_u64 4) u32)
+          <:
+          Core_models.Abstractions.Bitvec.t_BitVec (mk_u64 128)) ==
+        x)
+      [
+        SMTPat
+        (e_ee_14__impl__from_u32x4 (e_ee_14__impl__to_u32x4 x
+              <:
+              Core_models.Abstractions.Funarr.t_FunArray (mk_u64 4) u32)
+          <:
+          Core_models.Abstractions.Bitvec.t_BitVec (mk_u64 128))
+      ]
 
 unfold
 let e_ee_14__lemma_cancel_bv = e_ee_14__lemma_cancel_bv'
@@ -760,13 +984,21 @@ let e_ee_15__impl__to_u64x2 = e_ee_15__impl__to_u64x2'
 assume
 val e_ee_15__lemma_cancel_iv': x: Core_models.Abstractions.Funarr.t_FunArray (mk_u64 2) u64
   -> Lemma
-    (ensures
-      (e_ee_15__impl__to_u64x2 (e_ee_15__impl__from_u64x2 x
-            <:
-            Core_models.Abstractions.Bitvec.t_BitVec (mk_u64 128))
-        <:
-        Core_models.Abstractions.Funarr.t_FunArray (mk_u64 2) u64) ==
-      x)
+      (ensures
+        (e_ee_15__impl__to_u64x2 (e_ee_15__impl__from_u64x2 x
+              <:
+              Core_models.Abstractions.Bitvec.t_BitVec (mk_u64 128))
+          <:
+          Core_models.Abstractions.Funarr.t_FunArray (mk_u64 2) u64) ==
+        x)
+      [
+        SMTPat
+        (e_ee_15__impl__to_u64x2 (e_ee_15__impl__from_u64x2 x
+              <:
+              Core_models.Abstractions.Bitvec.t_BitVec (mk_u64 128))
+          <:
+          Core_models.Abstractions.Funarr.t_FunArray (mk_u64 2) u64)
+      ]
 
 unfold
 let e_ee_15__lemma_cancel_iv = e_ee_15__lemma_cancel_iv'
@@ -777,13 +1009,21 @@ let e_ee_15__lemma_cancel_iv = e_ee_15__lemma_cancel_iv'
 assume
 val e_ee_15__lemma_cancel_bv': x: Core_models.Abstractions.Bitvec.t_BitVec (mk_u64 128)
   -> Lemma
-    (ensures
-      (e_ee_15__impl__from_u64x2 (e_ee_15__impl__to_u64x2 x
-            <:
-            Core_models.Abstractions.Funarr.t_FunArray (mk_u64 2) u64)
-        <:
-        Core_models.Abstractions.Bitvec.t_BitVec (mk_u64 128)) ==
-      x)
+      (ensures
+        (e_ee_15__impl__from_u64x2 (e_ee_15__impl__to_u64x2 x
+              <:
+              Core_models.Abstractions.Funarr.t_FunArray (mk_u64 2) u64)
+          <:
+          Core_models.Abstractions.Bitvec.t_BitVec (mk_u64 128)) ==
+        x)
+      [
+        SMTPat
+        (e_ee_15__impl__from_u64x2 (e_ee_15__impl__to_u64x2 x
+              <:
+              Core_models.Abstractions.Funarr.t_FunArray (mk_u64 2) u64)
+          <:
+          Core_models.Abstractions.Bitvec.t_BitVec (mk_u64 128))
+      ]
 
 unfold
 let e_ee_15__lemma_cancel_bv = e_ee_15__lemma_cancel_bv'
@@ -812,13 +1052,21 @@ let e_ee_16__impl__to_u16x8 = e_ee_16__impl__to_u16x8'
 assume
 val e_ee_16__lemma_cancel_iv': x: Core_models.Abstractions.Funarr.t_FunArray (mk_u64 8) u16
   -> Lemma
-    (ensures
-      (e_ee_16__impl__to_u16x8 (e_ee_16__impl__from_u16x8 x
-            <:
-            Core_models.Abstractions.Bitvec.t_BitVec (mk_u64 128))
-        <:
-        Core_models.Abstractions.Funarr.t_FunArray (mk_u64 8) u16) ==
-      x)
+      (ensures
+        (e_ee_16__impl__to_u16x8 (e_ee_16__impl__from_u16x8 x
+              <:
+              Core_models.Abstractions.Bitvec.t_BitVec (mk_u64 128))
+          <:
+          Core_models.Abstractions.Funarr.t_FunArray (mk_u64 8) u16) ==
+        x)
+      [
+        SMTPat
+        (e_ee_16__impl__to_u16x8 (e_ee_16__impl__from_u16x8 x
+              <:
+              Core_models.Abstractions.Bitvec.t_BitVec (mk_u64 128))
+          <:
+          Core_models.Abstractions.Funarr.t_FunArray (mk_u64 8) u16)
+      ]
 
 unfold
 let e_ee_16__lemma_cancel_iv = e_ee_16__lemma_cancel_iv'
@@ -829,13 +1077,21 @@ let e_ee_16__lemma_cancel_iv = e_ee_16__lemma_cancel_iv'
 assume
 val e_ee_16__lemma_cancel_bv': x: Core_models.Abstractions.Bitvec.t_BitVec (mk_u64 128)
   -> Lemma
-    (ensures
-      (e_ee_16__impl__from_u16x8 (e_ee_16__impl__to_u16x8 x
-            <:
-            Core_models.Abstractions.Funarr.t_FunArray (mk_u64 8) u16)
-        <:
-        Core_models.Abstractions.Bitvec.t_BitVec (mk_u64 128)) ==
-      x)
+      (ensures
+        (e_ee_16__impl__from_u16x8 (e_ee_16__impl__to_u16x8 x
+              <:
+              Core_models.Abstractions.Funarr.t_FunArray (mk_u64 8) u16)
+          <:
+          Core_models.Abstractions.Bitvec.t_BitVec (mk_u64 128)) ==
+        x)
+      [
+        SMTPat
+        (e_ee_16__impl__from_u16x8 (e_ee_16__impl__to_u16x8 x
+              <:
+              Core_models.Abstractions.Funarr.t_FunArray (mk_u64 8) u16)
+          <:
+          Core_models.Abstractions.Bitvec.t_BitVec (mk_u64 128))
+      ]
 
 unfold
 let e_ee_16__lemma_cancel_bv = e_ee_16__lemma_cancel_bv'
